multi add

src/Dafny/examples/simple.i.dfy
@@ -20,33 +20,117 @@ lemma lvm_lemma_Empty_Test(lvm_b0:lvm_codes, lvm_s0:lvm_state, lvm_sN:lvm_state,
   ensures  lvm_get_ok(lvm_sM) // ValidState(sM)
   ensures  lvm_state_eq(lvm_sM, lvm_s0)
   ensures  lvm_state_eq(lvm_sM, lvm_update_mem( lvm_sM, lvm_update_ok(lvm_sM, lvm_sM)))
+  ensures  forall s2 :: evalCode(lvm_b0.hd, lvm_s0, s2,o) ==> s2.ok
 {
-  reveal_lvm_code_Empty_Test();
-  reveal_eval_code();
-  var lvm_old_s:lvm_state := lvm_s0;
+    reveal_lvm_code_Empty_Test();
+    reveal_eval_code();
+    var lvm_old_s:lvm_state := lvm_s0;
 
-  assert lvm_s0.ok;
-  assert lvm_code_Empty_Test() == Block(CNil);
-  assert lvm_b0.hd == lvm_code_Empty_Test();
-  assert !lvm_b0.CNil?;
-  assert lvm_code_Empty_Test().block.CNil?;
-  assert lvm_b0.hd.Block?;
-  assert lvm_get_block(lvm_b0.hd).CNil?;
-  assert evalBlock(lvm_get_block(lvm_b0.hd),lvm_s0, lvm_s0,o);
-  assert forall r :: r == lvm_s0 ==> eval_code(lvm_b0.hd,lvm_s0,r,o);
-  assert evalCode_lax(Block(lvm_b0), lvm_s0, lvm_sN, o);
+    assert lvm_s0.ok;
+    assert lvm_code_Empty_Test() == Block(CNil);
+    assert lvm_b0.hd == lvm_code_Empty_Test();
+    assert !lvm_b0.CNil?;
+    assert lvm_code_Empty_Test().block.CNil?;
+    assert lvm_b0.hd.Block?;
+    assert lvm_get_block(lvm_b0.hd).CNil?;
+    assert evalBlock(lvm_get_block(lvm_b0.hd),lvm_s0, lvm_s0,o);
+    assert forall r :: r == lvm_s0 ==> eval_code(lvm_b0.hd,lvm_s0,r,o);
+    assert evalCode_lax(Block(lvm_b0), lvm_s0, lvm_sN, o);
 
-  assert evalBlock(lvm_b0, lvm_s0, lvm_sN,o) ==> exists r' :: evalCode(lvm_b0.hd, lvm_s0, r',o) && evalBlock(lvm_b0.tl, r', lvm_sN,o);
-  assert exists r' :: if evalCode(lvm_b0.hd, lvm_s0, r',o) then true else true;
+    assert evalBlock(lvm_b0, lvm_s0, lvm_sN,o) ==> exists r' :: evalCode(lvm_b0.hd, lvm_s0, r',o) && evalBlock(lvm_b0.tl, r', lvm_sN,o);
+    assert exists r' :: if evalCode(lvm_b0.hd, lvm_s0, r',o) then true else true;
 
 
-  ghost var lvm_ltmp1, lvm_cM:lvm_code, lvm_ltmp2 := lvm_lemma_block_lax(lvm_b0, lvm_s0, lvm_sN,o);
-  lvm_sM := lvm_ltmp1;
-  lvm_bM := lvm_ltmp2;
-  var lvm_b1:lvm_codes := lvm_get_block(lvm_cM);
-  assert evalCode_lax(lvm_Block(lvm_CNil()), lvm_s0, lvm_sM, o);
+    ghost var lvm_ltmp1, lvm_cM:lvm_code, lvm_ltmp2 := lvm_lemma_block_lax(lvm_b0, lvm_s0, lvm_sN,o);
+    lvm_sM := lvm_ltmp1;
+    lvm_bM := lvm_ltmp2;
+    var lvm_b1:lvm_codes := lvm_get_block(lvm_cM);
+    assert evalCode_lax(lvm_Block(lvm_CNil()), lvm_s0, lvm_sM, o);
 
-  lvm_sM := lvm_lemma_empty(lvm_s0, lvm_sM);
+    lvm_sM := lvm_lemma_empty(lvm_s0, lvm_sM);
+}
+
+function method{:opaque}lvm_code_Add(dst:lvm_operand_opr, size:nat, src1:lvm_operand_opr,src2:lvm_operand_opr):lvm_code
+   requires src1.D?
+   requires src1.d.Int?
+   requires src2.D?
+   requires src2.d.Int?
+    requires typesMatch(src1.d,src2.d)
+
+{
+   Ins(ADD(dst, size,src1,src2))
+}
+lemma lvm_lemma_Add(lvm_b0:lvm_codes, lvm_s0:lvm_state, lvm_sN:lvm_state, 
+            dst:lvm_operand_opr, size:nat, src1:lvm_operand_opr,src2:lvm_operand_opr,o:operand)
+  returns (lvm_bM:lvm_codes, lvm_sM:lvm_state)
+  requires src1.D?
+  requires src1.d.Int?
+  requires src2.D?
+  requires src2.d.Int?
+  requires typesMatch(src1.d,src2.d)
+  requires lvm_require(lvm_b0, lvm_code_Add(dst, size,src1,src2), lvm_s0, lvm_sN,dst)
+  requires lvm_is_dst_opr(dst, lvm_s0)
+  requires lvm_is_src_opr(src1, lvm_s0)
+  requires lvm_get_ok(lvm_s0)
+
+  requires ValidOperand(lvm_s0,src1);
+  requires OperandContents(lvm_s0,src1).Int?;
+  requires ValidOperand(lvm_s0,src2);
+  requires OperandContents(lvm_s0,src2).Int?;
+  requires ValidOperand(lvm_s0,dst);
+  requires OperandContents(lvm_s0,dst).Int?;
+
+  requires ValidOperand(lvm_s0,dst);
+  requires typesMatch(OperandContents(lvm_s0,src1),OperandContents(lvm_s0,src2))
+  requires OperandContents(lvm_s0,src2).Int?;
+  requires lvm_code_Add(dst, size,src1,src2).Ins?;
+  requires ValidOperand(lvm_s0,dst)
+// //   
+  ensures  lvm_ensure(lvm_b0, lvm_bM, lvm_s0, lvm_sM, lvm_sN,dst)
+  ensures  lvm_get_ok(lvm_sM)
+  ensures  ValidOperand(lvm_sM,dst)
+  ensures  ValidOperand(lvm_sM,src1)
+  ensures OperandContents(lvm_sM,src1).Int?;
+  ensures  ValidOperand(lvm_sM,src2)
+  ensures OperandContents(lvm_sM,src2).Int?;
+  ensures typesMatch(OperandContents(lvm_sM,src1),OperandContents(lvm_sM,src2))
+
+  ensures  OperandContents(lvm_sM,dst).Int?;
+  ensures  lvm_state_eq(lvm_sM, lvm_update_mem( lvm_sM, lvm_update_all(lvm_sM, lvm_s0)))
+  ensures  lvm_state_eq(lvm_sM, lvm_update_ok(lvm_sM, lvm_update_all( lvm_sM, lvm_s0)))
+  ensures  forall s2 :: evalCode(lvm_b0.hd, lvm_s0, s2,o) ==> s2.ok
+  ensures OperandContents(lvm_sM, dst).val == evalADD(OperandContents(lvm_s0,dst).itype.size,OperandContents(lvm_s0,src1),OperandContents(lvm_s0,src2)).val;
+  ensures ToTwosComp(OperandContents(lvm_sM, dst)).val == 
+          (OperandContents(lvm_s0, src1).val + OperandContents(lvm_s0, src2).val) % Pow256(OperandContents(lvm_s0, src1).itype.size)
+
+{
+    reveal_lvm_code_Add();
+    reveal_evalCodeOpaque();
+    reveal_eval_code();
+    assert lvm_code_Add(dst, size,src1,src2).Ins?;
+    var addIns := lvm_code_Add(dst, size,src1,src2).ins;
+    assert ValidInstruction(lvm_s0,addIns);
+
+    assert  ValidRegOperand(lvm_s0, dst);
+    assert ValidState(lvm_s0);
+    var lvm_old_s:lvm_state := lvm_s0;
+    assert evalCode_lax(lvm_Block(lvm_b0), lvm_s0, lvm_sN,dst);
+    assert lvm_s0.ok;
+    assert eval_code(lvm_Block(lvm_b0), lvm_s0, lvm_sN,dst);
+
+    ghost var lvm_ltmp1, lvm_cM:lvm_code, lvm_ltmp2 := lvm_lemma_block(lvm_b0, lvm_s0, lvm_sN,dst);
+    lvm_sM := lvm_ltmp1;
+    lvm_bM := lvm_ltmp2;
+    assert lvm_b0.tl == lvm_bM;
+    assert ValidState(lvm_s0);
+    assert lvm_s0.ok;
+    assert ValidState(lvm_sM);
+    assert ValidOperand(lvm_sM,dst);
+    assert evalIns(lvm_code_Add(dst, size,src1,src2).ins,lvm_s0,lvm_sM,dst);
+    assert evalUpdate(lvm_s0, dst, evalADD(OperandContents(lvm_s0,dst).itype.size,OperandContents(lvm_s0,src1),OperandContents(lvm_s0,src2)),lvm_sM);
+    assert  ValidData(lvm_sM,evalADD(OperandContents(lvm_s0,dst).itype.size,OperandContents(lvm_s0,src1),OperandContents(lvm_s0,src2)));
+    assert OperandContents(lvm_sM, dst).val == evalADD(OperandContents(lvm_s0,dst).itype.size,OperandContents(lvm_s0,src1),OperandContents(lvm_s0,src2)).val;
+    reveal_evalCodeOpaque();
 }
 
 ////
@@ -61,7 +145,6 @@ function method{:opaque} lvm_code_Add_single(dst:lvm_operand_opr, size:nat, src1
     assert val.d.Int?;
     var void := D(Void);
     lvm_Block(lvm_CCons(Ins(ADD(dst, size,src1,val)),lvm_CNil()))
-
     // lvm_Block(lvm_CCons(Ins(ADD(dst, size,src1,val)),lvm_CCons(Ins(RET(void)),lvm_CNil())))
 
 }
@@ -69,6 +152,7 @@ function method{:opaque} lvm_code_Add_single(dst:lvm_operand_opr, size:nat, src1
 lemma lvm_lemma_Add_single(lvm_b0:lvm_codes, lvm_s0:lvm_state, lvm_sN:lvm_state, 
             dst:lvm_operand_opr, size:nat, src1:lvm_operand_opr,src2:lvm_operand_opr,o:operand)
   returns (lvm_bM:lvm_codes, lvm_sM:lvm_state)
+  requires src1.D?;
   requires lvm_require(lvm_b0, lvm_code_Add_single(dst, size,src1), lvm_s0, lvm_sN,dst)
   requires lvm_is_dst_opr(dst, lvm_s0)
   requires lvm_is_src_opr(src1, lvm_s0)
@@ -81,61 +165,64 @@ lemma lvm_lemma_Add_single(lvm_b0:lvm_codes, lvm_s0:lvm_state, lvm_sN:lvm_state,
 //   
   ensures  lvm_ensure(lvm_b0, lvm_bM, lvm_s0, lvm_sM, lvm_sN,dst)
   ensures  lvm_get_ok(lvm_sM)
-  ensures ValidOperand(lvm_sM,dst)
-  ensures OperandContents(lvm_sM,dst).Int?;
-  ensures OperandContents(lvm_s0,dst).Int?;
+  ensures  ValidOperand(lvm_sM,dst)
+  ensures  OperandContents(lvm_sM,dst).Int?;
+  ensures  OperandContents(lvm_s0,dst).Int?;
+  ensures  OperandContents(lvm_sM, dst).val == 
+  evalADD(OperandContents(lvm_s0,dst).itype.size,OperandContents(lvm_s0,src1),D(Int(4,src1.d.itype)).d).val;
   ensures  OperandContents(lvm_sM, dst).val == OperandContents(lvm_s0, dst).val + 4
-  ensures  lvm_state_eq(lvm_sM, lvm_update_ok(lvm_sM, lvm_update_mem( lvm_sM, lvm_s0)))
+  ensures  lvm_state_eq(lvm_sM, lvm_update_ok(lvm_sM, lvm_update_all( lvm_sM, lvm_s0)))
+  ensures  forall s2 :: evalCode(lvm_b0.hd, lvm_s0, s2,o) ==> s2.ok
+
 {
-  reveal_lvm_code_Add_single();
-  assert lvm_code_Add_single(dst, size,src1).Ins?;
-  var addIns := lvm_code_Add_single(dst, size,src1).ins;
-  assert ValidInstruction(lvm_s0,addIns);
+    reveal_lvm_code_Add_single();
+    assert lvm_code_Add_single(dst, size,src1).Ins?;
+    var addIns := lvm_code_Add_single(dst, size,src1).ins;
+    assert ValidInstruction(lvm_s0,addIns);
 
-  assert  ValidRegOperand(lvm_s0, dst);
-  assert ValidState(lvm_s0);
-  assert lvm_b0.hd.Ins?;
-  var lvm_old_s:lvm_state := lvm_s0;
-//   lvm_ins_lemma(Ins(InsAdd(dst, src)), lvm_s0);
-  ghost var lvm_ltmp1, lvm_cM:lvm_code, lvm_ltmp2 := lvm_lemma_block_lax(lvm_b0, lvm_s0, lvm_sN,dst);
-  lvm_sM := lvm_ltmp1;
-  lvm_bM := lvm_ltmp2;
-  assert lvm_b0.tl == lvm_bM;
-  assert lvm_bM.CNil?;
-//   assert  OperandContents(lvm_sM, dst).Int?;
+    assert  ValidRegOperand(lvm_s0, dst);
+    assert ValidState(lvm_s0);
+    assert lvm_b0.hd.Ins?;
+    var lvm_old_s:lvm_state := lvm_s0;
+    ghost var lvm_ltmp1, lvm_cM:lvm_code, lvm_ltmp2 := lvm_lemma_block(lvm_b0, lvm_s0, lvm_sN,dst);
+    lvm_sM := lvm_ltmp1;
+    lvm_bM := lvm_ltmp2;
+    assert lvm_b0.tl == lvm_bM;
+    assert lvm_bM.CNil?;
 
-  assert evalCode_lax(lvm_cM, lvm_s0, lvm_sM,dst);
-  assert OperandContents(lvm_sM, dst).val == OperandContents(lvm_s0, dst).val + 4;
+    assert evalCode_lax(lvm_cM, lvm_s0, lvm_sM,dst);
+    assert OperandContents(lvm_sM, dst).val == OperandContents(lvm_s0, dst).val + 4;
 
-  reveal_evalCodeOpaque();
+    reveal_evalCodeOpaque();
 }
 
-
-///
-function method lvm_code_Add_Multiple(lvm_s0:lvm_state,dst:lvm_operand_opr, size:nat, src1:lvm_operand_opr): (out:lvm_code)
+function method {:opaque} lvm_code_Add_Multiple(dst:lvm_operand_opr, size:nat, src1:lvm_operand_opr): (out:lvm_code)
+    requires src1.D?;
+    requires src1.d.Int?;
     ensures out.Block?;
     ensures out.block.lvm_CCons?;
     ensures out.block.hd.Ins?;
-    // ensures out.hd.Ins?;
-    // ensures ValidInstruction(lvm_s0,out.block.hd.ins);
+
 {
-    reveal_IntFits();
-    var val := D(Int(4,IntType(1,false)));
-    assert val.d.Int?;
-    var void := D(Void);
+      reveal_IntFits();
+      var val := D(Int(4,src1.d.itype));
+      assert val.d.Int?;
+      var void := D(Void);
 
-    var val2 := D(Int(5,IntType(1,false)));
-    assert val.d.Int?;
+      var val2 := D(Int(5,src1.d.itype));
+      assert val.d.Int?;
 
-    lvm_Block(lvm_CCons(Ins(ADD(dst,size,src1,val)),
-              lvm_CCons(Ins(ADD(dst,size,src1,val2)),lvm_CNil())))
+      lvm_Block(lvm_CCons(Ins(ADD(dst,size,src1,val)),
+                lvm_CCons(Ins(ADD(dst,size,src1,val2)),lvm_CNil())))
 
 }
 
 lemma lvm_lemma_Add_Multiple(lvm_b0:lvm_codes, lvm_s0:lvm_state, lvm_sN:lvm_state, 
             dst:lvm_operand_opr, size:nat, src1:lvm_operand_opr,src2:lvm_operand_opr,o:operand)
   returns (lvm_bM:lvm_codes, lvm_sM:lvm_state)
-  requires lvm_require(lvm_b0, lvm_code_Add_Multiple(lvm_s0,dst, size,src1).block.hd, lvm_s0, lvm_sN,dst)
+  requires src1.D?;
+  requires src1.d.Int?;
+  requires lvm_require(lvm_b0, lvm_code_Add_Multiple(dst, size,src1), lvm_s0, lvm_sN,dst)
   requires lvm_is_dst_opr(dst, lvm_s0)
   requires lvm_is_src_opr(src1, lvm_s0)
   requires lvm_get_ok(lvm_s0)
@@ -143,121 +230,78 @@ lemma lvm_lemma_Add_Multiple(lvm_b0:lvm_codes, lvm_s0:lvm_state, lvm_sN:lvm_stat
   requires ValidOperand(lvm_s0,src1);
   requires OperandContents(lvm_s0,src1).Int?;
   requires ValidOperand(lvm_s0,dst);
-  requires ValidInstruction(lvm_s0,lvm_code_Add_Multiple(lvm_s0,dst, size,src1).block.hd.ins);
-//   requires lvm_code_Add_Multiple(lvm_s0,dst, size,src1).Ins?; //  ISSUE <<---
+  requires ValidOperand(lvm_s0,dst);
+  requires OperandContents(lvm_s0,dst).Int?;
 
   requires ValidOperand(lvm_s0,dst)
 //   
   ensures  lvm_ensure(lvm_b0, lvm_bM, lvm_s0, lvm_sM, lvm_sN,dst)
   ensures  lvm_get_ok(lvm_sM) 
   ensures ValidOperand(lvm_sM,dst)
-
   ensures OperandContents(lvm_sM,dst).Int?;
   ensures OperandContents(lvm_s0,dst).Int?;
 
-  ensures  OperandContents(lvm_sM, dst).val == OperandContents(lvm_s0, dst).val + 9
-  ensures  lvm_state_eq(lvm_sM, lvm_update_ok(lvm_sM, lvm_update_mem( lvm_sM, lvm_s0)))
+  ensures  OperandContents(lvm_sM, dst).val == evalADD(OperandContents(lvm_s0,dst).itype.size,OperandContents(lvm_s0,src1),D(Int(5,src1.d.itype)).d).val;
+  ensures ToTwosComp(OperandContents(lvm_sM, dst)).val == 
+          (OperandContents(lvm_s0, src1).val + D(Int(5,src1.d.itype)).d.val) % Pow256(OperandContents(lvm_s0, src1).itype.size)
+  ensures  lvm_state_eq(lvm_sM, lvm_update_ok(lvm_sM, lvm_update_all( lvm_sM, lvm_s0)))
 {
-//   reveal_lvm_code_Add_Multiple();
-  assert lvm_code_Add_Multiple(lvm_s0,dst, size,src1).block.hd.Ins?;
-  var addIns := lvm_code_Add_Multiple(lvm_s0,dst, size,src1).block.hd.ins;
+    reveal_lvm_code_Add_Multiple();
+    reveal_eval_code();
+    reveal_evalCodeOpaque();
+    reveal_lvm_code_Add();
+    assert lvm_code_Add_Multiple(dst, size,src1).block.hd.Ins?;
 
-  assert ValidInstruction(lvm_s0,addIns);
-  assert  ValidRegOperand(lvm_s0, dst);
-  assert ValidState(lvm_s0);
-//   assert lvm_b0.block.hd.Ins?;
-  var lvm_old_s:lvm_state := lvm_s0;
-//   lvm_ins_lemma(Ins(InsAdd(dst, src)), lvm_s0);
-  ghost var lvm_ltmp1, lvm_cM:lvm_code, lvm_ltmp2 := lvm_lemma_block(lvm_b0, lvm_s0, lvm_sN,dst);
-  lvm_sM := lvm_ltmp1;
-  lvm_bM := lvm_ltmp2;
-  assert lvm_b0.tl == lvm_bM;
-//   assert lvm_bM.CNil?;
-//   assert  OperandContents(lvm_sM, dst).Int?;
+    assert ValidState(lvm_s0);
+    var lvm_old_s:lvm_state := lvm_s0;
+    assert evalCode(lvm_Block(lvm_b0), lvm_s0, lvm_sN,dst);
+    assert eval_code(lvm_Block(lvm_b0), lvm_s0, lvm_sN,dst);
 
-  assert evalCode_lax(lvm_cM, lvm_s0, lvm_sM,dst);
-  assert OperandContents(lvm_sM, dst).val == OperandContents(lvm_s0, dst).val + 4;
-//   assert ValidInstruction(lvm_s0,lvm_code_Add_Multiple(dst, size,src1,src2).ins) ==> lvm_sM.ok;
-//   assert evalUpdate(lvm_s0, o, evalADD(size,OperandContents(lvm_s0,src1),val), lvm_sM);
+    ghost var lvm_ltmp1, lvm_cM:lvm_code, lvm_ltmp2 := lvm_lemma_block(lvm_b0, lvm_s0, lvm_sN,dst);
+    lvm_sM := lvm_ltmp1;
+    lvm_bM := lvm_ltmp2;
+    var lvm_b1:lvm_codes := lvm_get_block(lvm_cM);
+    assert lvm_b1.lvm_CCons?;
+    reveal_IntFits();
+    var val := D(Int(4,src1.d.itype));
+    assert val.d.Int?;
+    assert lvm_b1.hd == lvm_code_Add(dst, size,src1,val);
+    assert ValidState(lvm_s0);
+    assert evalCode_lax(lvm_Block(lvm_b1), lvm_s0, lvm_sM,dst);
+    assert OperandContents(lvm_s0,dst).Int?;
 
-  reveal_evalCodeOpaque();
+    var val2 := D(Int(5,src1.d.itype));
+    var step1 := evalADD(OperandContents(lvm_s0,dst).itype.size,OperandContents(lvm_s0,src1),val.d);
+
+
+    ghost var lvm_b2, lvm_s2 := lvm_lemma_Add(lvm_b1, lvm_s0, lvm_sM, dst, size,src1,val,o);
+
+
+    assert OperandContents(lvm_s2, dst).val == step1.val;
+    assert OperandContents(lvm_s0, src1) == OperandContents(lvm_s2, src1); 
+
+    assert  lvm_require(lvm_b2, lvm_code_Add(dst, size,src1,val2), lvm_s2, lvm_sM,dst);
+    var step2 := evalADD(OperandContents(lvm_s2,dst).itype.size,OperandContents(lvm_s2,src1),val2.d);
+
+    ghost var lvm_b3, lvm_s3 := lvm_lemma_Add(lvm_b2, lvm_s2, lvm_sM, dst, size,src1,val2,o);
+    assert OperandContents(lvm_s3, dst).val 
+        == evalADD(OperandContents(lvm_s2,dst).itype.size,OperandContents(lvm_s2,src1),val2.d).val;
+  
+    assert OperandContents(lvm_s3, dst).val  == step2.val;
+    assert lvm_b3.CNil?;
+    lvm_sM := lvm_lemma_empty(lvm_s3,lvm_sM);
+    assert   OperandContents(lvm_sM, dst).val  == step2.val;
+
+    assert evalCode_lax(lvm_cM, lvm_s0, lvm_sM,dst);
+        assert OperandContents(lvm_s0, src1) == OperandContents(lvm_sM, src1); 
+
+    assert OperandContents(lvm_sM, dst).val == step2.val;
+    assert  OperandContents(lvm_sM, dst).val == evalADD(OperandContents(lvm_s0,dst).itype.size,OperandContents(lvm_s0,src1),val2.d).val;
+    assert ValidState(lvm_sM);
+
+    reveal_evalCodeOpaque();
 }
 
-
-
-// function method{:opaque} lvm_code_Add(dst:lvm_operand_opr, size:nat, src1:lvm_operand_opr): (out:lvm_code)
-//     ensures out.Block?;
-//     ensures out.block.lvm_CCons?;
-//     ensures out.block.hd.Ins?;
-// {
-//     reveal_IntFits();
-//     var val := D(Int(4,IntType(1,false)));
-//     assert val.d.Int?;
-//     var void := D(Void);
-//     lvm_Block(lvm_CCons(Ins(ADD(dst, size,src1,val)),lvm_CCons(Ins(RET(void)),lvm_CNil())))
-
-// }
-
-// lemma lvm_lemma_Add(lvm_b0:lvm_codes, lvm_s0:lvm_state, lvm_sN:lvm_state, 
-//             dst:lvm_operand_opr, size:nat, src1:lvm_operand_opr,src2:lvm_operand_opr,o:operand)
-//   returns (lvm_bM:lvm_codes, lvm_sM:lvm_state)
-//   requires lvm_require(lvm_b0, lvm_code_Add(dst, size,src1), lvm_s0, lvm_sN,dst)
-//   requires lvm_is_dst_opr(dst, lvm_s0)
-//   requires lvm_is_src_opr(src1, lvm_s0)
-//   requires lvm_get_ok(lvm_s0)
-
-//   requires ValidOperand(lvm_s0,src1);
-//   requires OperandContents(lvm_s0,src1).Int?;
-//   requires ValidInstruction(lvm_s0,lvm_code_Add(dst, size,src1).block.hd.ins);
-// //   requires lvm_code_Add(dst, size,src1).Ins?;
-
-// //   requires dst.GV?;
-//   requires ValidOperand(lvm_s0,dst)
-// //   
-//   ensures  lvm_ensure(lvm_b0, lvm_bM, lvm_s0, lvm_sM, lvm_sN,dst)
-//   ensures  lvm_get_ok(lvm_sM)
-//   ensures ValidOperand(lvm_sM,dst)
-
-//   ensures OperandContents(lvm_sM,dst).Int?;
-//   ensures OperandContents(lvm_s0,dst).Int?;
-
-//   ensures  OperandContents(lvm_sM, dst).val == OperandContents(lvm_s0, dst).val + 4
-//   ensures  lvm_state_eq(lvm_sM, lvm_update_ok(lvm_sM, lvm_update_mem( lvm_sM, lvm_s0)))
-// {
-//     // assert dst.g in lvm_s0.gvs;
-//   reveal_lvm_code_Add();
-//   assert lvm_code_Add(dst, size,src1).Block?;
-//   var addIns := lvm_code_Add(dst, size,src1).block.hd.ins;
-//   assert ValidInstruction(lvm_s0,addIns);
-// //   assert o == dst;
-//   assert  ValidRegOperand(lvm_s0, dst);
-//   assert ValidOperand(lvm_s0,dst);
-//   assert ValidState(lvm_s0);
-//   assert lvm_b0.hd.Block?;
-//   assert lvm_b0.hd == lvm_code_Add(dst, size,src1);
-// //   assert lvm_b0.hd.Ins?;
-//   var lvm_old_s:lvm_state := lvm_s0;
-// //   lvm_ins_lemma(Ins(InsAdd(dst, src)), lvm_s0);
-//   ghost var lvm_ltmp1, lvm_cM:lvm_code, lvm_ltmp2 := lvm_lemma_block_lax(lvm_b0, lvm_s0, lvm_sN,dst);
-//   lvm_sM := lvm_ltmp1;
-//   lvm_bM := lvm_ltmp2;
-//   assert lvm_b0.tl == lvm_bM;
-//   assert lvm_cM == lvm_b0.hd;
-// //   assert lvm_bM.CNil?;
-// //   assert  OperandContents(lvm_sM, dst).Int?;
-
-//   assert evalCode_lax(lvm_cM, lvm_s0, lvm_sM,dst);
-//   assert lvm_s0.ok;
-//   assert lvm_cM.block.hd.Ins?;
-//   assert exists r' :: evalCode(lvm_cM.block.hd,lvm_s0,r',dst);
-//   assert evalBlock(lvm_cM.block,lvm_s0, lvm_sM,dst);
-
-//   assert OperandContents(lvm_sM, dst).val == OperandContents(lvm_s0, dst).val + 4;
-// //   assert ValidInstruction(lvm_s0,lvm_code_Add(dst, size,src1,src2).ins) ==> lvm_sM.ok;
-// //   assert evalUpdate(lvm_s0, o, evalADD(size,OperandContents(lvm_s0,src1),val), lvm_sM);
-
-//   reveal_evalCodeOpaque();
-// }
 
 
 }
