src/Dafny/Operations/binaryOperations.i.dfy
@@ -11,28 +11,101 @@ module binary_operations_i {
         requires isInt(v0)
         requires isInt(v1)
         requires typesMatch(v0,v1)
-        // ensures out.itype.size == size
+        requires validBitWidth(v0.itype.size)
+        ensures out.Int?
+        ensures validBitWidth(out.itype.size)
+        ensures ToTwosComp(out).val == (v0.val + v1.val) % Pow256(v0.itype.size)
     { 
         reveal_ToTwosComp();
         reveal_FromTwosComp();
-        if (v0.itype.size == 1 && !v0.itype.signed) then UInt8(BitwiseAdd8(DataToUInt8(ToTwosComp(v0)),DataToUInt8(ToTwosComp(v1)))) else 
-        if (v0.itype.size == 1 && v0.itype.signed) then FromTwosComp(UInt8(BitwiseAdd8(DataToUInt8(ToTwosComp(v1)),DataToUInt8(ToTwosComp(v0))))) else 
-        if (v0.itype.size == 2 && !v0.itype.signed) then UInt16(BitwiseAdd16(DataToUInt16(ToTwosComp(v0)),DataToUInt16(ToTwosComp(v1)))) else 
-        if (v0.itype.size == 2 && v0.itype.signed) then FromTwosComp(UInt16(BitwiseAdd16(DataToUInt16(ToTwosComp(v1)),DataToUInt16(ToTwosComp(v0))))) else 
-        if (v0.itype.size == 4 && !v0.itype.signed) then UInt32(BitwiseAdd32(DataToUInt32(ToTwosComp(v0)),DataToUInt32(ToTwosComp(v1)))) else 
-        if (v0.itype.size == 4 && v0.itype.signed) then FromTwosComp(UInt32(BitwiseAdd32(DataToUInt32(ToTwosComp(v1)),DataToUInt32(ToTwosComp(v0))))) else 
-        if (v0.itype.size == 8 && !v0.itype.signed) then UInt64(BitwiseAdd64(DataToUInt64(ToTwosComp(v0)),DataToUInt64(ToTwosComp(v1)))) else 
-        if (v0.itype.size == 8 && v0.itype.signed) then FromTwosComp(UInt64(BitwiseAdd64(DataToUInt64(ToTwosComp(v1)),DataToUInt64(ToTwosComp(v0))))) else v0
-
+        if (v0.itype.size == 1) then evalADD8(size,v0,v1) else
+        if (v0.itype.size == 2) then evalADD16(size,v0,v1) else
+        if (v0.itype.size == 4) then evalADD32(size,v0,v1) else
+                                     evalADD64(size,v0,v1)
     }
 
+    function evalADD8(size:nat,v0:Data,v1:Data):  (out:Data)
+        requires isInt(v0)
+        requires isInt(v1)
+        requires typesMatch(v0,v1)
+        requires validBitWidth(v0.itype.size)
+        requires v0.itype.size == 1
+        ensures out.Int?
+        ensures validBitWidth(out.itype.size)
+        ensures (!v0.itype.signed) ==> out.val == (v0.val + v1.val) % 0x100
+        ensures (v0.itype.signed) ==> ToTwosComp(out).val == (v0.val + v1.val) % 0x100
+        
+        {
+            reveal_ToTwosComp();
+            reveal_FromTwosComp();
+            if (!v0.itype.signed) then UInt8(BitwiseAdd8(DataToUInt8(ToTwosComp(v0)),DataToUInt8(ToTwosComp(v1)))) else 
+                                       FromTwosComp(UInt8(BitwiseAdd8(DataToUInt8(ToTwosComp(v1)),DataToUInt8(ToTwosComp(v0)))))  
+        }
+
+    function evalADD16(size:nat,v0:Data,v1:Data):  (out:Data)
+        requires isInt(v0)
+        requires isInt(v1)
+        requires typesMatch(v0,v1)
+        requires validBitWidth(v0.itype.size)
+        requires v0.itype.size == 2
+        ensures out.Int?
+        ensures validBitWidth(out.itype.size)
+        ensures (!v0.itype.signed) ==> out.val == (v0.val + v1.val) % 0x10000
+        ensures (v0.itype.signed) ==> ToTwosComp(out).val == (v0.val + v1.val) % 0x10000
+        
+        {
+            reveal_ToTwosComp();
+            reveal_FromTwosComp();
+            if (!v0.itype.signed) then UInt16(BitwiseAdd16(DataToUInt16(ToTwosComp(v0)),DataToUInt16(ToTwosComp(v1)))) else 
+                                       FromTwosComp(UInt16(BitwiseAdd16(DataToUInt16(ToTwosComp(v1)),DataToUInt16(ToTwosComp(v0)))))
+        }
+
+    function evalADD32(size:nat,v0:Data,v1:Data):  (out:Data)
+        requires isInt(v0)
+        requires isInt(v1)
+        requires typesMatch(v0,v1)
+        requires validBitWidth(v0.itype.size)
+        requires v0.itype.size == 4
+        ensures out.Int?
+        ensures validBitWidth(out.itype.size)
+        ensures (!v0.itype.signed) ==> out.val == (v0.val + v1.val) % 0x1_0000_0000
+        ensures (v0.itype.signed) ==> ToTwosComp(out).val == (v0.val + v1.val) % 0x1_0000_0000
+        
+        {
+            reveal_ToTwosComp();
+            reveal_FromTwosComp();
+            if (!v0.itype.signed) then UInt32(BitwiseAdd32(DataToUInt32(ToTwosComp(v0)),DataToUInt32(ToTwosComp(v1)))) else  
+                                       FromTwosComp(UInt32(BitwiseAdd32(DataToUInt32(ToTwosComp(v1)),DataToUInt32(ToTwosComp(v0)))))
+        }
+
+    function evalADD64(size:nat,v0:Data,v1:Data):  (out:Data)
+        requires isInt(v0)
+        requires isInt(v1)
+        requires typesMatch(v0,v1)
+        requires validBitWidth(v0.itype.size)
+        requires v0.itype.size == 8
+        ensures out.Int?
+        ensures validBitWidth(out.itype.size)
+        ensures (!v0.itype.signed) ==> out.val == (v0.val + v1.val) % 0x1_0000_0000_0000_0000
+        ensures (v0.itype.signed) ==> ToTwosComp(out).val == (v0.val + v1.val) % 0x1_0000_0000_0000_0000
+        
+        {
+            reveal_ToTwosComp();
+            reveal_FromTwosComp();
+            if (!v0.itype.signed) then UInt64(BitwiseAdd64(DataToUInt64(ToTwosComp(v0)),DataToUInt64(ToTwosComp(v1)))) else  
+                                       FromTwosComp(UInt64(BitwiseAdd64(DataToUInt64(ToTwosComp(v1)),DataToUInt64(ToTwosComp(v0)))))
+        }
 
     function evalSUB(size:nat,v0:Data,v1:Data):  (out:Data) // doesnt support nsw/nuw
         requires isInt(v0)
         requires isInt(v1)
         requires typesMatch(v0,v1)
+        requires validBitWidth(v0.itype.size)
+        ensures out.Int?
         // ensures out.itype.size == size
         ensures (v0.itype.size == 1 && v0.itype.signed) ==> evalSUB(size,v0,v1)== FromTwosComp(UInt8(BitwiseSub8(DataToUInt8(ToTwosComp(v1)),DataToUInt8(ToTwosComp(v0)))))
+        // ensures ToTwosComp(out).val == (v0.val - v1.val) % Pow256(v0.itype.size)
+
     { 
         reveal_ToTwosComp();
         reveal_FromTwosComp();
@@ -43,9 +116,28 @@ module binary_operations_i {
         if (v0.itype.size == 4 && !v0.itype.signed) then UInt32(BitwiseSub32(DataToUInt32(ToTwosComp(v0)),DataToUInt32(ToTwosComp(v1)))) else 
         if (v0.itype.size == 4 && v0.itype.signed) then FromTwosComp(UInt32(BitwiseSub32(DataToUInt32(ToTwosComp(v1)),DataToUInt32(ToTwosComp(v0))))) else 
         if (v0.itype.size == 8 && !v0.itype.signed) then UInt64(BitwiseSub64(DataToUInt64(ToTwosComp(v0)),DataToUInt64(ToTwosComp(v1)))) else 
-        if (v0.itype.size == 8 && v0.itype.signed) then FromTwosComp(UInt64(BitwiseSub64(DataToUInt64(ToTwosComp(v1)),DataToUInt64(ToTwosComp(v0))))) else v0
+        FromTwosComp(UInt64(BitwiseSub64(DataToUInt64(ToTwosComp(v1)),DataToUInt64(ToTwosComp(v0)))))
 
     }
+
+    // function evaSUB8(size:nat,v0:Data,v1:Data):  (out:Data)
+    //     requires isInt(v0)
+    //     requires isInt(v1)
+    //     requires typesMatch(v0,v1)
+    //     requires validBitWidth(v0.itype.size)
+    //     requires v0.itype.size == 1
+    //     ensures out.Int?
+    //     ensures validBitWidth(out.itype.size)
+    //     ensures (!v0.itype.signed) ==> out.val == (v0.val - v1.val) % 0x100
+    //     // ensures (v0.itype.signed) ==> ToTwosComp(out).val == (v0.val - v1.val) % 0x100
+        
+    //     {
+    //         reveal_ToTwosComp();
+    //         reveal_FromTwosComp();
+    //         if (!v0.itype.signed) then UInt8(BitwiseSub8(DataToUInt8(ToTwosComp(v0)),DataToUInt8(ToTwosComp(v1)))) else 
+    //                                    FromTwosComp(UInt8(BitwiseSub8(DataToUInt8(ToTwosComp(v1)),DataToUInt8(ToTwosComp(v0)))))  
+    //     }
+
 
 //-----------------------------------------------------------------------------
 // INSTRICTION VALIDITY
@@ -158,6 +250,7 @@ lemma evalSUB8check_signed()
         var v3:sint8 := -50;
         assert SInt8(v2).itype.size == 1 && SInt8(v2).itype.signed;
         assert FromTwosComp(UInt8(BitwiseSub8(DataToUInt8(ToTwosComp(SInt8(v2))),DataToUInt8(ToTwosComp(SInt8(v3)))))).val == 52;
+            //    FromTwosComp(UInt8(BitwiseSub8(DataToUInt8(ToTwosComp(v1)),DataToUInt8(ToTwosComp(v0)))))
         assert evalSUB(1,SInt8(v2),SInt8(v3)).val == -52;
         
         assert -evalSUB(1,SInt8(v2),SInt8(v3)).val == FromTwosComp(UInt8(BitwiseSub8(DataToUInt8(ToTwosComp(SInt8(v2))),DataToUInt8(ToTwosComp(SInt8(v3)))))).val;
